src/coq/STsep.v
@@ -34,45 +34,54 @@ Require Import Ynot.Util.
 Require Import Ynot.Heap.
 Require Import Ynot.Hprop.
 Require Import Ynot.ST.
+Require Import Qcanon.
 
 Set Implicit Arguments.
 
-
 Notation "{{{ v }}}" := (STWeaken _ (STStrengthen _ v _) _) (at level 0).
 
+Local Open Scope hprop_scope.
+
 Definition STsep pre T (post : T -> hprop) : Type :=
-  ST (pre * ??) (fun h v h' =>
+  ST ((pre *! ??) & total_heap) (fun h v h' =>
     forall h1 h2, h ~> h1 * h2
-      -> pre h1
-      -> exists h1', h' ~> h1' * h2
+      -> total_heap h
+      -> (h1 <*> h2)%heap
+      -> pre h1 
+      -> exists h1', h' ~> h1' * h2 
+        /\ total_heap h'
+        /\ (h1' <*> h2)%heap
         /\ post v h1').
 
 Arguments Scope STsep [hprop_scope type_scope hprop_scope].
 
-
 Ltac hreduce :=
   repeat match goal with
            | [ |- (hprop_inj _) _ ] => red
-           | [ |- (hprop_cell _ _) _ ] => red
+           | [ |- (hprop_cell _ _ _) _ ] => red
            | [ |- (hprop_sep _ _) _ ] => red
+           | [ |- (hprop_and _ _) _ ] => red
+           | [ |- (hprop_sep_valid _ _) _ ] => red
            | [ |- hprop_empty _ ] => red
            | [ |- hprop_any _ ] => red
            | [ |- (hprop_ex _) _ ] => red
 
            | [ H : (hprop_inj _) _ |- _ ] => red in H
-           | [ H : (hprop_cell _ _) _ |- _ ] => red in H
+           | [ H : (hprop_cell _ _ _) _ |- _ ] => red in H
            | [ H : (hprop_sep _ _) _ |- _ ] => red in H
+           | [ H : (hprop_and _ _) _ |- _ ] => red in H
+           | [ H : (hprop_sep_valid _ _) _ |- _ ] => red in H
            | [ H : hprop_empty _ |- _ ] => red in H
            | [ H : hprop_any _ |- _ ] => clear H
            | [ H : (hprop_ex _) _ |- _ ] => destruct H
 
            | [ H : ex _ |- _ ] => destruct H
 
-           | [ H : _ ~> empty * _ |- _ ] => generalize (split_id1_invert H); clear H
+           | [ H : _ ~> empty * _ |- _ ] => generalize (split_id_invert H); clear H
          end.
 
 Hint Extern 1 ((hprop_inj _) _) => hreduce : Ynot.
-Hint Extern 1 ((hprop_cell _ _) _) => hreduce : Ynot.
+Hint Extern 1 ((hprop_cell _ _ _) _) => hreduce : Ynot.
 Hint Extern 1 ((hprop_sep _ _) _) => hreduce : Ynot.
 Hint Extern 1 (hprop_empty _) => hreduce : Ynot.
 Hint Extern 1 (hprop_any _) => hreduce : Ynot.
@@ -84,8 +93,10 @@ Section Sep.
 
   Definition SepReturn T (v : T) : STsep __ (fun v' => [v' = v])%hprop.
     t.
-    refine {{{STReturn v}}}; ynot 7.
+    refine {{{STReturn v}}}; ynot 8.
   Qed.
+
+  Local Open Scope hprop_scope.
 
   Definition SepBind pre1 T1 (post1 : T1 -> hprop)
     pre2 T2 (post2 : T2 -> hprop)
@@ -96,17 +107,17 @@ Section Sep.
     unfold hprop_imp; t.
 
     refine (STBind _ _ _ _ st1 st2 _ _ _).
-
     tauto.
+    intros.
 
-    ynot 1.
-    generalize (H1 _ _ H2); clear H1.
-    ynot 7.
+    ynot 1;
+    generalize (H1 _ _ H2); clear H1;
+    ynot 8.
 
     ynot 1.
     generalize (H1 _ _ H4 H5); clear H1.
     ynot 1.
-    generalize (H3 _ _ H8); clear H3.
+    generalize (H3 _ _ H14); clear H3.
     ynot 1.
   Qed.
 
@@ -132,41 +143,157 @@ Section Sep.
     t.
     exact (STFix _ _ _ F v).
   Qed.
-  
+
+  Lemma split_read_total0none h h1 h2 d p : 
+    h ~> h1 * h2 
+    -> (total_heap h 
+    -> h1 <*> h2
+    -> h1 # p = Some (d, 0)
+    -> h2 # p = None)%heap.
+  Proof.
+    intros. generalize (H0 p).
+    generalize (split_read1 p H H2). generalize (H1 p).
+    intros. 
+    rewrite H2 in H3. unfold read in *. simpl in *.
+    rewrite H4 in H5. simpl in *.
+    unfold add_qopl in *. destruct (h2 p); trivial.
+    rewrite Qcplus_0_l in H5.
+    rewrite H5 in H3. intuition.
+  Qed.
+
+  Lemma split_read_total0 h h1 h2 d p : 
+    h ~> h1 * h2 
+    -> (total_heap h 
+    -> h1 # p = Some (d, 0)
+    -> h # p = Some (d, 0))%heap.
+  Proof.
+    intros.
+    generalize (split_read1 p H H1). unfold read. simpl. intro.
+    generalize (H0 p). rewrite H2. simpl. congruence.
+  Qed.
+
+  Hint Resolve split_read_total0 : Ynot.
+    
+  Hint Resolve total_heap_new total_heap_free : Ynot.
+
+  Lemma free_none_eq h p : (h # p = None -> h ### p = h)%heap.
+  Proof.
+    unfold read, free, heap. intros. ext_eq.
+    destruct (ptr_eq_dec x p); congruence.
+  Qed.
+
+  Hint Resolve free_none_eq : Ynot.
+
+  (* automate more of this stuff *)
+  Lemma split_free_total0 h h1 h2 d p :
+    h ~> h1 * h2
+    -> ((total_heap h)
+    -> h1 <*> h2
+    -> (h1 # p) = Some (d, 0)
+    -> (h2 ### p) = h2)%heap.
+    Proof.
+      unfold free, heap.
+      intros. ext_eq.
+      destruct (ptr_eq_dec x p); trivial.
+      subst.
+      generalize (split_read_total0none p H H0 H1 H2).
+      ynot 1.
+    Qed.
+
+    Lemma valid_join_new h A (v:A) p q : ((h # p) = None ->  (p |--> (Dyn v, q)) <*> h)%heap.
+    Proof.
+     unfold heap, singleton, join_valid, read. simpl. intros. 
+     destruct (ptr_eq_dec p0 p); trivial. subst. rewrite H. trivial.
+    Qed.
+
+    Hint Resolve valid_join_new : Ynot.
+
   Definition SepNew (T : Set) (v : T)
-    : STsep __ (fun p => p --> v)%hprop.
+    : STsep __ (fun p => p -0-> v)%hprop.
     t.
-    refine {{{STNew v}}}; ynot 8.
+    refine {{{STNew v}}}; ynot 5.
+    eexists. intuition.
   Qed.
 
   Definition SepFree T p
-    : STsep (Exists v :@ T, p --> v)%hprop (fun _ : unit => __)%hprop.
+    : STsep (Exists v :@ T, p -0-> v)%hprop (fun _ : unit => __)%hprop.
     t.
     refine {{{STFree p}}}; ynot 5.
+    eexists. intuition. 
+    generalize (split_free H1 H H6). intro.
+    ynot 2. rewrite H7.
+    rewrite (split_free_total0 p H1); ynot 1.
   Qed.
 
-  Definition SepRead (T : Set) (p : ptr) (P : T -> hprop)
-    : STsep (Exists v :@ T, p --> v * P v)%hprop (fun v => p --> v * P v)%hprop.
+
+  Theorem Dynq_inj_Someq : forall (T : Set) (x y : T) (q1 q2 : Qc),
+    Some (Dyn x, q1) = Some (Dyn y, q2)
+    -> q1 = q2.
+    intros. inversion H. trivial.
+  Qed.
+
+  Lemma Dynq_inj_Somed' : forall (d1 d2 : dynamic) (q : Qc),
+    Some (d1, q) = Some (d2, q)
+    -> d1 = d2.
+    congruence.
+  Qed.
+  
+  Theorem Dynq_inj_Somed : forall (T : Set) (x y : T) (q1 q2 : Qc),
+    Some (Dyn x, q1) = Some (Dyn y, q2)
+    -> x = y.
+    intros. inversion H. subst.
+    apply Dyn_inj.
+    apply Dynq_inj_Somed' with (q:=q2).
+    trivial.
+  Qed.
+
+  (* this should be automated *)
+  Definition SepRead (T : Set) (p : ptr) (P : T -> hprop) (q:[Qc])
+    : STsep (Exists v :@ T, (q ~~ p -[q]-> v * P v))%hprop (fun v => (q ~~ p -[q]-> v * P v))%hprop.
     t.
     refine {{{STRead T p}}}; ynot 5.
 
-    rewrite (split2_read _ H0 H H1) in H2.
-    generalize (Dyn_inj_Some H2); clear H2; intro; subst.
+    destruct H2. intuition. subst.
+    ynot 2.
+    rewrite (split2_read p H0 H3 H4). simpl. 
+    eauto.
 
-    ynot 10.
+
+    exists h1. intuition.
+    replace v with x; trivial.
+    destruct H1. intuition. destruct H9.
+    destruct H1. intuition.
+    destruct H1.
+    generalize (split2_read p H0 H9 H1).
+    rewrite H2. simpl. intro.
+
+    generalize (Dynq_inj_Somed H12); auto. 
   Qed.
 
+  Lemma join_valid_update h1 h2 p d d' :
+    h1 <*> h2 
+    -> (h1 # p = Some (d, 0)
+    -> (h1 ## p <- (d', 0)) <*> h2)%heap.
+  Proof.
+    unfold join_valid, write, read. intros.
+    generalize (H p). generalize (H p0). rewrite H0. unfold read. 
+    destruct (ptr_eq_dec p0 p); subst; trivial.
+  Qed.
+
+  Hint Resolve split_read_total0none : Ynot.
+  Hint Resolve join_valid_update : Ynot.
+
   Definition SepWrite (T T' : Set) (p : ptr) (v : T')
-    : STsep (Exists v' :@ T, p --> v')%hprop (fun _ : unit => p --> v)%hprop.
+    : STsep (Exists v' :@ T, p -0-> v')%hprop (fun _ : unit => p -0-> v)%hprop.
     t.
     refine {{{STWrite T p v}}}; ynot 5.
 
-    exists (h1 ## p <- Dyn v)%heap; intuition.
-    eauto with Ynot.
-    red; intuition.
-    autorewrite with Ynot.
-    unfold read in H4.
-    auto.
+    exists (h1 ## p <- (Dyn v,0))%heap; intuition.
+    ynot 3.
+    ynot 2.
+    ynot 1.
+    unfold write, read in H6 |- *.
+    destruct (ptr_eq_dec p' p); intuition.
   Qed.
 
   Definition SepStrengthen pre T (post : T -> hprop) (pre' : hpre)
@@ -174,7 +301,7 @@ Section Sep.
     : pre' ==> pre
     -> STsep pre' post.
     unfold hprop_imp; t.
-    refine {{{st}}}; ynot 7.
+    refine {{{st}}}; ynot 8.
   Qed.
 
   Definition SepWeaken pre T (post post' : T -> hprop)
@@ -184,13 +311,118 @@ Section Sep.
     unfold hprop_imp; t.
     refine {{{st}}}; ynot 1.
 
-    generalize (H1 _ _ H2); clear H1; ynot 4.
+    generalize (H1 _ _ H2); clear H1; ynot 6.
   Qed.
+
+(*
+  Lemma join_valid_splice h x x0 x1 x2 :
+    total_heap h
+    -> (h ~> x * x0)
+    -> (x <*> x0)
+    -> (x ~> x1 * x2)
+    -> x2 <*> (x0 * x1).
+  Proof.
+    intros.
+    assert (h ~> x2 * (x0 * x1)).
+    eauto with Ynot.
+    
+    intro.
+    generalize (H p). clear H.  intro H.
+    generalize (H1 p). clear H1. intro H1.
+
+    destruct H3. destruct H2. subst. unfold join, read in *.
+    destruct (x2 p); destruct (x0 p); destruct (x1 p); simpl in *.
+    intuition.
+    rewrite H5 in *.
+    rewrite Qcplus_0_l in H4.
+
+*)
 
   Definition SepFrame pre T (post : T -> hprop) (st : STsep pre post) (P : hprop)
     : STsep (P * pre) (fun v => P * post v)%hprop.
     t.
-    refine {{{st}}}; ynot 7.
+    refine {{{st}}}; ynot 7. 
+    assert (h ~> x2 * (x0 * x1)).
+    eauto with Ynot.
+
+    (* arg! this is more annoying *)
+    eexists. eexists. split.
+    2: repeat split.
+    3: eauto. eauto.
+    
+
+    
+    
+    destruct H3. subst.
+    destruct H0. subst.
+    split_prover'.
+    unfold join, read in *.
+
+    destruct (x2 p); trivial.
+    destruct (x0 p); destruct (x1 p); simpl in *.
+    intuition. destruct h; destruct h0; destruct h1; simpl in *. subst.
+    
+    rewrite Qcplus_0_r in *.
+    simpl in *.
+    destruct
+    
+    clear H4 H6 pre st post T P.
+    destruct H3. subst. clear H5.
+    destruct H0. subst.
+    (* HERE *)
+    intro.
+    split_prover'.
+    unfold read, join in *.
+    destruct (x0 p); destruct (x1 p); destruct (x2 p); simpl in *; trivial.
+    intuition; trivial.
+    destruct h0; destruct h1; destruct h; simpl in *; subst; trivial.
+    rewrite Qcplus_0_r in *. subst.
+
+    
+    generalize (H p); clear H. intro H.
+    generalize (H1 p); clear H1. intro H1.
+    generalize (H2 p); clear H2. intro H2.
+    unfold join, read in *.
+
+    intuition.
+
+    
+    
+
+    Focus 2.
+    assert (h ~> x4 * (x1 * x3)).
+    eauto with Ynot.
+
+    generalize (H0 _ _ H7); clear H0; ynot 0.
+    exists (x5 * x)%heap; ynot 3.
+    
+    x0.
+
+    exists x.
+    exists x5.
+    intuition.
+    eauto with Ynot.
+
+
+
+    exists x2. exists ((x0 * x1)%heap). intuition.
+    
+    (* lemma me *)
+
+
+    -> h ~> x2 * (x0 * x1)
+    -> 
+    -> h
+
+
+    generalize (H0 _ _ H6); clear H0; ynot 0.
+    exists (x5 * x)%heap; ynot 3.
+
+    exists x.
+    exists x5.
+    intuition.
+    eauto with Ynot.
+
 
     assert (h ~> x0 * (h2 * x)).
     eauto with Ynot.
